Remove names

theories/Equality.v
@@ -7,96 +7,8 @@ Section Equality.
 Context `{Sort_notion : Sorts.notion}.
 
 (*! Equality between terms *)
-(* This goes through the definition of a nameless syntax *)
 
-Inductive nlterm : Type :=
-| nlRel (n : nat)
-| nlSort (s : sort)
-| nlProd (A B : nlterm)
-| nlLambda (A B t : nlterm)
-| nlApp (u : nlterm) (A B v : nlterm)
-(* Σ-types *)
-| nlSum (A B : nlterm)
-| nlPair (A B u v : nlterm)
-| nlPi1 (A B p : nlterm)
-| nlPi2 (A B p : nlterm)
-(* Homogenous equality *)
-| nlEq (A u v : nlterm)
-| nlRefl (A u : nlterm)
-| nlJ (A u P w v p : nlterm)
-| nlTransport (T1 T2 p t : nlterm)
-| nlBeta (f t : nlterm)
-(* Heterogenous equality *)
-| nlHeq (A a B b : nlterm)
-| nlHeqToEq (p : nlterm)
-| nlHeqRefl (A a : nlterm)
-| nlHeqSym (p : nlterm)
-| nlHeqTrans (p q : nlterm)
-| nlHeqTransport (p t : nlterm)
-| nlCongProd (B1 B2 pA pB : nlterm)
-| nlCongLambda (B1 B2 t1 t2 pA pB pt : nlterm)
-| nlCongApp (B1 B2 pu pA pB pv : nlterm)
-| nlCongSum (B1 B2 pA pB : nlterm)
-| nlCongPair (B1 B2 pA pB pu pv : nlterm)
-| nlCongPi1 (B1 B2 pA pB pp : nlterm)
-| nlCongPi2 (B1 B2 pA pB pp : nlterm)
-| nlCongEq (pA pu pv : nlterm)
-| nlCongRefl (pA pu : nlterm)
-| nlEqToHeq (p : nlterm)
-| nlHeqTypeEq (A B p : nlterm)
-(* Packing *)
-| nlPack (A1 A2 : nlterm)
-| nlProjT1 (p : nlterm)
-| nlProjT2 (p : nlterm)
-| nlProjTe (p : nlterm)
-(* External axioms *)
-| nlAx (id : ident)
-.
-
-Fixpoint nl (t : sterm) : nlterm :=
-  match t with
-  | sRel n => nlRel n
-  | sSort s => nlSort s
-  | sProd n A B => nlProd (nl A) (nl B)
-  | sLambda n A B t => nlLambda (nl A) (nl B) (nl t)
-  | sApp u A B v => nlApp (nl u) (nl A) (nl B) (nl v)
-  | sSum n A B => nlSum (nl A) (nl B)
-  | sPair A B u v => nlPair (nl A) (nl B) (nl u) (nl v)
-  | sPi1 A B p => nlPi1 (nl A) (nl B) (nl p)
-  | sPi2 A B p => nlPi2 (nl A) (nl B) (nl p)
-  | sEq A u v => nlEq (nl A) (nl u) (nl v)
-  | sRefl A u => nlRefl (nl A) (nl u)
-  | sJ A u P w v p => nlJ (nl A) (nl u) (nl P) (nl w) (nl v) (nl p)
-  | sTransport T1 T2 p t => nlTransport (nl T1) (nl T2) (nl p) (nl t)
-  | sBeta f t => nlBeta (nl f) (nl t)
-  | sHeq A a B b => nlHeq (nl A) (nl a) (nl B) (nl b)
-  | sHeqToEq p => nlHeqToEq (nl p)
-  | sHeqRefl A a => nlHeqRefl (nl A) (nl a)
-  | sHeqSym p => nlHeqSym (nl p)
-  | sHeqTrans p q => nlHeqTrans (nl p) (nl q)
-  | sHeqTransport p t => nlHeqTransport (nl p) (nl t)
-  | sCongProd B1 B2 pA pB => nlCongProd (nl B1) (nl B2) (nl pA) (nl pB)
-  | sCongLambda B1 B2 t1 t2 pA pB pt =>
-    nlCongLambda (nl B1) (nl B2) (nl t1) (nl t2) (nl pA) (nl pB) (nl pt)
-  | sCongApp B1 B2 pu pA pB pv =>
-    nlCongApp (nl B1) (nl B2) (nl pu) (nl pA) (nl pB) (nl pv)
-  | sCongSum B1 B2 pA pB => nlCongSum (nl B1) (nl B2) (nl pA) (nl pB)
-  | sCongPair B1 B2 pA pB pu pv =>
-    nlCongPair (nl B1) (nl B2) (nl pA) (nl pB) (nl pu) (nl pv)
-  | sCongPi1 B1 B2 pA pB pp => nlCongPi1 (nl B1) (nl B2) (nl pA) (nl pB) (nl pp)
-  | sCongPi2 B1 B2 pA pB pp => nlCongPi2 (nl B1) (nl B2) (nl pA) (nl pB) (nl pp)
-  | sCongEq pA pu pv => nlCongEq (nl pA) (nl pu) (nl pv)
-  | sCongRefl pA pu => nlCongRefl (nl pA) (nl pu)
-  | sEqToHeq p => nlEqToHeq (nl p)
-  | sHeqTypeEq A B p => nlHeqTypeEq (nl A) (nl B) (nl p)
-  | sPack A1 A2 => nlPack (nl A1) (nl A2)
-  | sProjT1 p => nlProjT1 (nl p)
-  | sProjT2 p => nlProjT2 (nl p)
-  | sProjTe p => nlProjTe (nl p)
-  | sAx id => nlAx id
-  end.
-
-Section nldec.
+Section dec.
 
   Ltac finish :=
     let h := fresh "h" in
@@ -108,36 +20,36 @@ Section nldec.
 
   Ltac fcase c :=
     let e := fresh "e" in
-    case c ; intro e ; [subst ; try (left ; reflexivity) | finish].
+    case c ; intro e ; [ subst ; try (left ; reflexivity) | finish ].
 
-  Ltac nl_dec_tac nl_dec :=
+  Ltac dec_tac dec :=
     repeat match goal with
-           | t : nlterm, u : nlterm |- _ => fcase (nl_dec t u)
+           | t : sterm, u : sterm |- _ => fcase (dec t u)
            | s : sort, z : sort |- _ => fcase (Sorts.eq_dec s z)
            | n : nat, m : nat |- _ => fcase (Nat.eq_dec n m)
            | i : ident, i' : ident |- _ => fcase (string_dec i i')
            end.
 
-  Fixpoint nl_dec (t u : nlterm) : { t = u } + { t <> u }.
+  Fixpoint eq_term_dec (t u : sterm) : { t = u } + { t <> u }.
   Proof.
     destruct t ; destruct u ; try (right ; discriminate).
-    all: nl_dec_tac nl_dec.
+    all: dec_tac eq_term_dec.
   Defined.
 
-End nldec.
+End dec.
 
 Definition eq_term (t u : sterm) : bool :=
-  if nl_dec (nl t) (nl u) then true else false.
+  if eq_term_dec t u then true else false.
 
 Lemma eq_term_spec :
   forall {t u},
-    eq_term t u = true <-> nl t = nl u.
+    eq_term t u = true <-> t = u.
 Proof.
   intros t u. split.
-  - unfold eq_term. case (nl_dec (nl t) (nl u)).
+  - unfold eq_term. case (eq_term_dec t u).
     + intros. assumption.
     + intros. discriminate.
-  - unfold eq_term. case (nl_dec (nl t) (nl u)).
+  - unfold eq_term. case (eq_term_dec t u).
     + reflexivity.
     + intros h e. exfalso. apply h. apply e.
 Defined.
@@ -146,7 +58,7 @@ Fact eq_term_refl :
   forall {t}, eq_term t t = true.
 Proof.
   intro t. unfold eq_term.
-  case (nl_dec (nl t) (nl t)).
+  case (eq_term_dec t t).
   - intro. reflexivity.
   - intro h. exfalso. apply h. reflexivity.
 Defined.
@@ -156,9 +68,9 @@ Fact eq_term_sym :
 Proof.
   unfold eq_term.
   intros t u.
-  case (nl_dec (nl u) (nl t)) ; intro e.
+  case (eq_term_dec u t) ; intro e.
   - reflexivity.
-  - case (nl_dec (nl t) (nl u)) ; intro e'.
+  - case (eq_term_dec t u) ; intro e'.
     + exfalso. apply e. easy.
     + intro. easy.
 Defined.
@@ -168,26 +80,9 @@ Fact eq_term_trans :
 Proof.
   intros t u v.
   unfold eq_term.
-  case (nl_dec (nl t) (nl u)) ; intro e1.
+  case (eq_term_dec t u) ; intro e1.
   - intros _. rewrite e1. auto.
   - discriminate.
-Defined.
-
-Lemma nl_lift :
-  forall {t u n k},
-    nl t = nl u ->
-    nl (lift n k t) = nl (lift n k u).
-Proof.
-  intros t u n k.
-  case (nl_dec (nl t) (nl u)).
-  - intros e _.
-    revert u e n k.
-    induction t ;
-    intros u e m k ; destruct u ; cbn in e ; try discriminate e.
-    all:
-      try (cbn ; inversion e ;
-           repeat (erewrite_assumption by eassumption) ; reflexivity).
-  - intros h e. exfalso. apply h. apply e.
 Defined.
 
 Lemma eq_term_lift :
@@ -197,30 +92,10 @@ Lemma eq_term_lift :
 Proof.
   intros t u n k h. apply eq_term_spec in h.
   apply eq_term_spec.
-  apply nl_lift. assumption.
+  f_equal. assumption.
 Defined.
 
-Lemma nl_subst :
-  forall {t t' u u' n},
-    nl t = nl t' ->
-    nl u = nl u' ->
-    nl (t{n := u}) = nl (t'{n := u'}).
-Proof.
-  intros t t' u u' n ht hu. revert t' ht u u' hu n.
-  induction t ;
-  intros t' ht.
-  all: destruct t' ; cbn in ht ; try discriminate ht.
-  all: intros u u' hu m.
-  all: try (cbn ; inversion ht ;
-            repeat (erewrite_assumption by eassumption) ; reflexivity).
-  symmetry in ht. inversion ht. subst. clear ht. cbn.
-  case_eq (m ?= n) ; intro e ; bprop e.
-  + subst. eapply nl_lift. assumption.
-  + reflexivity.
-  + reflexivity.
-Defined.
-
-Corollary eq_term_subst :
+Lemma eq_term_subst :
   forall {t t' u u' n},
     eq_term t t' = true ->
     eq_term u u' = true ->
@@ -230,7 +105,7 @@ Proof.
   apply eq_term_spec in ht.
   apply eq_term_spec in hu.
   apply eq_term_spec.
-  apply nl_subst ; assumption.
+  f_equal. all: assumption.
 Defined.
 
 End Equality.
