theories/WEquality.v
@@ -6,66 +6,9 @@ Section Equality.
 
 Context `{Sort_notion : Sorts.notion}.
 
-(*! Equality between terms *)
-(* This goes through the definition of a nameless syntax *)
+(* Equality between terms *)
 
-Inductive nlterm : Type :=
-| nlRel (n : nat)
-| nlSort (s : sort)
-| nlProd (A B : nlterm)
-| nlLambda (A t : nlterm)
-| nlApp (u v : nlterm)
-(* Σ-types *)
-| nlSum (A B : nlterm)
-| nlPair (A B u v : nlterm)
-| nlPi1 (A B p : nlterm)
-| nlPi2 (A B p : nlterm)
-(* Homogenous equality *)
-| nlEq (A u v : nlterm)
-| nlRefl (A u : nlterm)
-| nlJ (A u P w v p : nlterm)
-| nlTransport (A B p t : nlterm)
-| nlBeta (f t : nlterm)
-| nlK (A u p : nlterm)
-| nlFunext (f g p : nlterm)
-| nlJBeta (u P w : nlterm)
-| nlTransportBeta (A t : nlterm)
-| nlPairEta (p : nlterm)
-| nlProdExt (A p : nlterm)
-| nlSumExt (A p : nlterm)
-(* External axioms *)
-| nlAx (id : ident)
-| nlDelta (id : ident)
-.
-
-Fixpoint nl (t : wterm) : nlterm :=
-  match t with
-  | wRel n => nlRel n
-  | wSort s => nlSort s
-  | wProd n A B => nlProd (nl A) (nl B)
-  | wLambda n A t => nlLambda (nl A) (nl t)
-  | wApp u v => nlApp (nl u) (nl v)
-  | wSum n A B => nlSum (nl A) (nl B)
-  | wPair A B u v => nlPair (nl A) (nl B) (nl u) (nl v)
-  | wPi1 A B p => nlPi1 (nl A) (nl B) (nl p)
-  | wPi2 A B p => nlPi2 (nl A) (nl B) (nl p)
-  | wEq A u v => nlEq (nl A) (nl u) (nl v)
-  | wRefl A u => nlRefl (nl A) (nl u)
-  | wJ A u P w v p => nlJ (nl A) (nl u) (nl P) (nl w) (nl v) (nl p)
-  | wTransport T1 T2 p t => nlTransport (nl T1) (nl T2) (nl p) (nl t)
-  | wBeta f t => nlBeta (nl f) (nl t)
-  | wK A u p => nlK (nl A) (nl u) (nl p)
-  | wFunext f g p => nlFunext (nl f) (nl g) (nl p)
-  | wJBeta u P w => nlJBeta (nl u) (nl P) (nl w)
-  | wTransportBeta A t => nlTransportBeta (nl A) (nl t)
-  | wPairEta p => nlPairEta (nl p)
-  | wProdExt A p => nlProdExt (nl A) (nl p)
-  | wSumExt A p => nlSumExt (nl A) (nl p)
-  | wAx id => nlAx id
-  | wDelta id => nlDelta id
-  end.
-
-Section nldec.
+Section dec.
 
   Ltac finish :=
     let h := fresh "h" in
@@ -77,36 +20,36 @@ Section nldec.
 
   Ltac fcase c :=
     let e := fresh "e" in
-    case c ; intro e ; [subst ; try (left ; reflexivity) | finish].
+    case c ; intro e ; [ subst ; try (left ; reflexivity) | finish ].
 
-  Ltac nl_dec_tac nl_dec :=
+  Ltac eq_term_dec_tac eq_term_dec :=
     repeat match goal with
-           | t : nlterm, u : nlterm |- _ => fcase (nl_dec t u)
+           | t : wterm, u : wterm |- _ => fcase (eq_term_dec t u)
            | s : sort, z : sort |- _ => fcase (Sorts.eq_dec s z)
            | n : nat, m : nat |- _ => fcase (Nat.eq_dec n m)
            | i : ident, i' : ident |- _ => fcase (string_dec i i')
            end.
 
-  Fixpoint nl_dec (t u : nlterm) : { t = u } + { t <> u }.
+  Fixpoint eq_term_dec (t u : wterm) : { t = u } + { t <> u }.
   Proof.
     destruct t ; destruct u ; try (right ; discriminate).
-    all: nl_dec_tac nl_dec.
+    all: eq_term_dec_tac eq_term_dec.
   Defined.
 
-End nldec.
+End dec.
 
 Definition eq_term (t u : wterm) : bool :=
-  if nl_dec (nl t) (nl u) then true else false.
+  if eq_term_dec t u then true else false.
 
 Lemma eq_term_spec :
   forall {t u},
-    eq_term t u = true <-> nl t = nl u.
+    eq_term t u = true <-> t = u.
 Proof.
   intros t u. split.
-  - unfold eq_term. case (nl_dec (nl t) (nl u)).
+  - unfold eq_term. case (eq_term_dec t u).
     + intros. assumption.
     + intros. discriminate.
-  - unfold eq_term. case (nl_dec (nl t) (nl u)).
+  - unfold eq_term. case (eq_term_dec t u).
     + reflexivity.
     + intros h e. exfalso. apply h. apply e.
 Defined.
@@ -115,7 +58,7 @@ Fact eq_term_refl :
   forall {t}, eq_term t t = true.
 Proof.
   intro t. unfold eq_term.
-  case (nl_dec (nl t) (nl t)).
+  case (eq_term_dec t t).
   - intro. reflexivity.
   - intro h. exfalso. apply h. reflexivity.
 Defined.
@@ -125,9 +68,9 @@ Fact eq_term_sym :
 Proof.
   unfold eq_term.
   intros t u.
-  case (nl_dec (nl u) (nl t)) ; intro e.
+  case (eq_term_dec u t) ; intro e.
   - reflexivity.
-  - case (nl_dec (nl t) (nl u)) ; intro e'.
+  - case (eq_term_dec t u) ; intro e'.
     + exfalso. apply e. easy.
     + intro. easy.
 Defined.
@@ -137,26 +80,9 @@ Fact eq_term_trans :
 Proof.
   intros t u v.
   unfold eq_term.
-  case (nl_dec (nl t) (nl u)) ; intro e1.
+  case (eq_term_dec t u) ; intro e1.
   - intros _. rewrite e1. auto.
   - discriminate.
-Defined.
-
-Lemma nl_lift :
-  forall {t u n k},
-    nl t = nl u ->
-    nl (lift n k t) = nl (lift n k u).
-Proof.
-  intros t u n k.
-  case (nl_dec (nl t) (nl u)).
-  - intros e _.
-    revert u e n k.
-    induction t ;
-    intros u e m k ; destruct u ; cbn in e ; try discriminate e.
-    all:
-      try (cbn ; inversion e ;
-           repeat (erewrite_assumption by eassumption) ; reflexivity).
-  - intros h e. exfalso. apply h. apply e.
 Defined.
 
 Lemma eq_term_lift :
@@ -166,30 +92,10 @@ Lemma eq_term_lift :
 Proof.
   intros t u n k h. apply eq_term_spec in h.
   apply eq_term_spec.
-  apply nl_lift. assumption.
+  f_equal. assumption.
 Defined.
 
-Lemma nl_subst :
-  forall {t t' u u' n},
-    nl t = nl t' ->
-    nl u = nl u' ->
-    nl (t{n := u}) = nl (t'{n := u'}).
-Proof.
-  intros t t' u u' n ht hu. revert t' ht u u' hu n.
-  induction t ;
-  intros t' ht.
-  all: destruct t' ; cbn in ht ; try discriminate ht.
-  all: intros u u' hu m.
-  all: try (cbn ; inversion ht ;
-            repeat (erewrite_assumption by eassumption) ; reflexivity).
-  symmetry in ht. inversion ht. subst. clear ht. cbn.
-  case_eq (m ?= n) ; intro e ; bprop e.
-  + subst. eapply nl_lift. assumption.
-  + reflexivity.
-  + reflexivity.
-Defined.
-
-Corollary eq_term_subst :
+Lemma eq_term_subst :
   forall {t t' u u' n},
     eq_term t t' = true ->
     eq_term u u' = true ->
@@ -199,7 +105,7 @@ Proof.
   apply eq_term_spec in ht.
   apply eq_term_spec in hu.
   apply eq_term_spec.
-  apply nl_subst ; assumption.
+  f_equal. all: assumption.
 Defined.
 
 End Equality.
