theories/ITypingInversions.v
@@ -36,14 +36,8 @@ Ltac invtac :=
   intros ;
   lazymatch goal with
   | h : _ |- _ =>
-    dependent induction h ; [
-      repeat eexists ; eassumption
-    | destruct_pands ; mysplits ; try eassumption ;
-      match goal with
-      | h : nl ?A = _ |- _ =>
-        solve [ transitivity (nl A) ; eauto ]
-      end
-    ]
+    dependent induction h ;
+    repeat eexists ; eassumption
   end.
 
 Lemma inversionRel :
@@ -51,7 +45,7 @@ Lemma inversionRel :
     Σ ;;; Γ |-i sRel n : T ->
     exists A,
       nth_error Γ n = Some A /\
-      nl (lift0 (S n) A) = nl T.
+      lift0 (S n) A = T.
 Proof.
   invtac.
 Defined.
@@ -59,30 +53,30 @@ Defined.
 Lemma inversionSort :
   forall {Σ Γ s T},
     Σ ;;; Γ |-i sSort s : T ->
-    nl (sSort (Sorts.succ s)) = nl T.
+    sSort (Sorts.succ s) = T.
 Proof.
   invtac.
 Defined.
 
 Lemma inversionProd :
-  forall {Σ Γ n A B T},
-    Σ ;;; Γ |-i sProd n A B : T ->
+  forall {Σ Γ A B T},
+    Σ ;;; Γ |-i sProd A B : T ->
     exists s1 s2,
       (Σ ;;; Γ |-i A : sSort s1) /\
       (Σ ;;; Γ ,, A |-i B : sSort s2) /\
-      (nl (sSort (Sorts.prod_sort s1 s2)) = nl T).
+      (sSort (Sorts.prod_sort s1 s2) = T).
 Proof.
   invtac.
 Defined.
 
 Lemma inversionLambda :
-  forall {Σ Γ na A B t T},
-    Σ ;;; Γ |-i sLambda na A B t : T ->
-      exists s1 s2 na',
+  forall {Σ Γ A B t T},
+    Σ ;;; Γ |-i sLambda A B t : T ->
+      exists s1 s2,
         (Σ ;;; Γ |-i A : sSort s1) /\
         (Σ ;;; Γ ,, A |-i B : sSort s2) /\
         (Σ ;;; Γ ,, A |-i t : B) /\
-        (nl (sProd na' A B) = nl T).
+        (sProd A B = T).
 Proof.
   invtac.
 Defined.
@@ -90,23 +84,23 @@ Defined.
 Lemma inversionApp :
   forall {Σ Γ t A B u T},
     Σ ;;; Γ |-i sApp t A B u : T ->
-    exists s1 s2 n,
+    exists s1 s2,
       (Σ ;;; Γ |-i A : sSort s1) /\
       (Σ ;;; Γ ,, A |-i B : sSort s2) /\
-      (Σ ;;; Γ |-i t : sProd n A B) /\
+      (Σ ;;; Γ |-i t : sProd A B) /\
       (Σ ;;; Γ |-i u : A) /\
-      (nl (B{ 0 := u }) = nl T).
+      (B{ 0 := u } = T).
 Proof.
   invtac.
 Defined.
 
 Lemma inversionSum :
-  forall {Σ Γ n A B T},
-    Σ ;;; Γ |-i sSum n A B : T ->
+  forall {Σ Γ A B T},
+    Σ ;;; Γ |-i sSum A B : T ->
     exists s1 s2,
       (Σ ;;; Γ |-i A : sSort s1) /\
       (Σ ;;; Γ ,, A |-i B : sSort s2) /\
-      (nl (sSort (Sorts.sum_sort s1 s2)) = nl T).
+      (sSort (Sorts.sum_sort s1 s2) = T).
 Proof.
   invtac.
 Defined.
@@ -114,12 +108,12 @@ Defined.
 Lemma inversionPair :
   forall {Σ Γ A B u v T},
     Σ ;;; Γ |-i sPair A B u v : T ->
-    exists n s1 s2,
+    exists s1 s2,
       (Σ ;;; Γ |-i A : sSort s1) /\
       (Σ ;;; Γ ,, A |-i B : sSort s2) /\
       (Σ ;;; Γ |-i u : A) /\
       (Σ ;;; Γ |-i v : B{ 0 := u }) /\
-      (nl (sSum n A B) = nl T).
+      (sSum A B = T).
 Proof.
   invtac.
 Defined.
@@ -127,11 +121,11 @@ Defined.
 Lemma inversionPi1 :
   forall {Σ Γ A B p T},
     Σ ;;; Γ |-i sPi1 A B p : T ->
-    exists n s1 s2,
-      (Σ ;;; Γ |-i p : sSum n A B) /\
+    exists s1 s2,
+      (Σ ;;; Γ |-i p : sSum A B) /\
       (Σ ;;; Γ |-i A : sSort s1) /\
       (Σ ;;; Γ ,, A |-i B : sSort s2) /\
-      (nl A = nl T).
+      (A = T).
 Proof.
   invtac.
 Defined.
@@ -139,11 +133,11 @@ Defined.
 Lemma inversionPi2 :
   forall {Σ Γ A B p T},
     Σ ;;; Γ |-i sPi2 A B p : T ->
-    exists n s1 s2,
-      (Σ ;;; Γ |-i p : sSum n A B) /\
+    exists s1 s2,
+      (Σ ;;; Γ |-i p : sSum A B) /\
       (Σ ;;; Γ |-i A : sSort s1) /\
       (Σ ;;; Γ ,, A |-i B : sSort s2) /\
-      (nl (B{ 0 := sPi1 A B p }) = nl T).
+      (B{ 0 := sPi1 A B p } = T).
 Proof.
   invtac.
 Defined.
@@ -155,7 +149,7 @@ Lemma inversionEq :
       (Σ ;;; Γ |-i A : sSort s) /\
       (Σ ;;; Γ |-i u : A) /\
       (Σ ;;; Γ |-i v : A) /\
-      (nl (sSort (Sorts.eq_sort s)) = nl T).
+      (sSort (Sorts.eq_sort s) = T).
 Proof.
   invtac.
 Defined.
@@ -166,7 +160,7 @@ Lemma inversionRefl :
     exists s,
       (Σ ;;; Γ |-i A : sSort s) /\
       (Σ ;;; Γ |-i u : A) /\
-      (nl (sEq A u u) = nl T).
+      (sEq A u u = T).
 Proof.
   invtac.
 Defined.
@@ -181,7 +175,7 @@ Lemma inversionJ :
       (Σ ;;; Γ ,, A ,, (sEq (lift0 1 A) (lift0 1 u) (sRel 0)) |-i P : sSort s2) /\
       (Σ ;;; Γ |-i p : sEq A u v) /\
       (Σ ;;; Γ |-i w : (P {1 := u}){0 := sRefl A u}) /\
-      (nl (P{1 := v}{0 := p}) = nl T).
+      (P{1 := v}{0 := p} = T).
 Proof.
   invtac.
 Defined.
@@ -194,7 +188,7 @@ Lemma inversionTransport :
       (Σ ;;; Γ |-i t : A) /\
       (Σ ;;; Γ |-i A : sSort s) /\
       (Σ ;;; Γ |-i B : sSort s) /\
-      (nl B = nl T).
+      (B = T).
 Proof.
   invtac.
 Defined.
@@ -202,12 +196,11 @@ Defined.
 Lemma inversionBeta :
   forall {Σ Γ t u T},
     Σ ;;; Γ |-i sBeta t u : T ->
-    exists s n A B,
+    exists s A B,
       (Σ ;;; Γ,, A |-i t : B) /\
       (Σ ;;; Γ |-i u : A) /\
       (Σ ;;; Γ |-i A : sSort s) /\
-      (nl (sEq (B {0 := u}) (sApp (sLambda n A B t) A B u) (t {0 := u}))
-       = nl T).
+      (sEq (B {0 := u}) (sApp (sLambda A B t) A B u) (t {0 := u}) = T).
 Proof.
   invtac.
 Defined.
@@ -220,7 +213,7 @@ Lemma inversionHeq :
       (Σ ;;; Γ |-i B : sSort s) /\
       (Σ ;;; Γ |-i a : A) /\
       (Σ ;;; Γ |-i b : B) /\
-      (nl (sSort (heq_sort s)) = nl T).
+      (sSort (heq_sort s) = T).
 Proof.
   invtac.
 Defined.
@@ -231,7 +224,7 @@ Lemma inversionPack :
     exists s,
       (Σ ;;; Γ |-i A1 : sSort s) /\
       (Σ ;;; Γ |-i A2 : sSort s) /\
-      (nl (sSort (pack_sort s)) = nl T).
+      (sSort (pack_sort s) = T).
 Proof.
   invtac.
 Defined.
@@ -244,7 +237,7 @@ Lemma inversionHeqToEq :
      (Σ ;;; Γ |-i A : sSort s) /\
      (Σ ;;; Γ |-i u : A) /\
      (Σ ;;; Γ |-i v : A) /\
-     (nl (sEq A u v) = nl T).
+     (sEq A u v = T).
 Proof.
   invtac.
 Defined.
@@ -255,7 +248,7 @@ Lemma inversionHeqRefl :
     exists s,
       (Σ ;;; Γ |-i A : sSort s) /\
       (Σ ;;; Γ |-i a : A) /\
-      (nl (sHeq A a A a) = nl T).
+      (sHeq A a A a = T).
 Proof.
   invtac.
 Defined.
@@ -269,7 +262,7 @@ Lemma inversionHeqSym :
       (Σ ;;; Γ |-i b : B) /\
       (Σ ;;; Γ |-i A : sSort s) /\
       (Σ ;;; Γ |-i B : sSort s) /\
-      (nl (sHeq B b A a) = nl T).
+      (sHeq B b A a = T).
 Proof.
   invtac.
 Defined.
@@ -286,7 +279,7 @@ Lemma inversionHeqTrans :
       (Σ ;;; Γ |-i A : sSort s) /\
       (Σ ;;; Γ |-i B : sSort s) /\
       (Σ ;;; Γ |-i C : sSort s) /\
-      (nl (sHeq A a C c) = nl T).
+      (sHeq A a C c = T).
 Proof.
   invtac.
 Defined.
@@ -299,7 +292,7 @@ Lemma inversionHeqTransport :
       (Σ ;;; Γ |-i t : A) /\
       (Σ ;;; Γ |-i A : sSort s) /\
       (Σ ;;; Γ |-i B : sSort s) /\
-      (nl (sHeq A t B (sTransport A B p t)) = nl T).
+      (sHeq A t B (sTransport A B p t) = T).
 Proof.
   invtac.
 Defined.
@@ -307,7 +300,7 @@ Defined.
 Lemma inversionCongProd :
   forall {Σ Γ B1 B2 pA pB T},
     Σ ;;; Γ |-i sCongProd B1 B2 pA pB : T ->
-    exists s z nx ny A1 A2,
+    exists s z A1 A2,
       (Σ ;;; Γ |-i pA : sHeq (sSort s) A1 (sSort s) A2) /\
       (Σ ;;; Γ ,, (sPack A1 A2)
        |-i pB : sHeq (sSort z) ((lift 1 1 B1){ 0 := sProjT1 (sRel 0) })
@@ -316,17 +309,15 @@ Lemma inversionCongProd :
       (Σ ;;; Γ |-i A2 : sSort s) /\
       (Σ ;;; Γ ,, A1 |-i B1 : sSort z) /\
       (Σ ;;; Γ ,, A2 |-i B2 : sSort z) /\
-      (nl (sHeq (sSort (Sorts.prod_sort s z)) (sProd nx A1 B1)
-                (sSort (Sorts.prod_sort s z)) (sProd ny A2 B2))
-       = nl T).
+      (sHeq (sSort (Sorts.prod_sort s z)) (sProd A1 B1) (sSort (Sorts.prod_sort s z)) (sProd A2 B2) = T).
 Proof.
-  invtac. Unshelve. all: constructor.
+  invtac.
 Defined.
 
 Lemma inversionCongLambda :
   forall {Σ Γ B1 B2 t1 t2 pA pB pt T},
     Σ ;;; Γ |-i sCongLambda B1 B2 t1 t2 pA pB pt : T ->
-    exists s z nx ny A1 A2,
+    exists s z A1 A2,
       (Σ ;;; Γ |-i pA : sHeq (sSort s) A1 (sSort s) A2) /\
       (Σ ;;; Γ ,, (sPack A1 A2)
        |-i pB : sHeq (sSort z) ((lift 1 1 B1){ 0 := sProjT1 (sRel 0) })
@@ -342,34 +333,30 @@ Lemma inversionCongLambda :
       (Σ ;;; Γ ,, A2 |-i B2 : sSort z) /\
       (Σ ;;; Γ ,, A1 |-i t1 : B1) /\
       (Σ ;;; Γ ,, A2 |-i t2 : B2) /\
-      (nl (sHeq (sProd nx A1 B1) (sLambda nx A1 B1 t1)
-                (sProd ny A2 B2) (sLambda ny A2 B2 t2))
-       = nl T).
+      (sHeq (sProd A1 B1) (sLambda A1 B1 t1) (sProd A2 B2) (sLambda A2 B2 t2) = T).
 Proof.
-  invtac. Unshelve. all: constructor.
+  invtac.
 Defined.
 
 Lemma inversionCongApp :
   forall {Σ Γ B1 B2 pu pA pB pv T},
     Σ ;;; Γ |-i sCongApp B1 B2 pu pA pB pv : T ->
-    exists s z nx ny A1 A2 u1 u2 v1 v2,
+    exists s z A1 A2 u1 u2 v1 v2,
       (Σ ;;; Γ |-i pA : sHeq (sSort s) A1 (sSort s) A2) /\
       (Σ ;;; Γ ,, (sPack A1 A2)
        |-i pB : sHeq (sSort z) ((lift 1 1 B1){ 0 := sProjT1 (sRel 0) })
                     (sSort z) ((lift 1 1 B2){ 0 := sProjT2 (sRel 0) })) /\
-      (Σ ;;; Γ |-i pu : sHeq (sProd nx A1 B1) u1 (sProd ny A2 B2) u2) /\
+      (Σ ;;; Γ |-i pu : sHeq (sProd A1 B1) u1 (sProd A2 B2) u2) /\
       (Σ ;;; Γ |-i pv : sHeq A1 v1 A2 v2) /\
       (Σ ;;; Γ |-i A1 : sSort s) /\
       (Σ ;;; Γ |-i A2 : sSort s) /\
       (Σ ;;; Γ ,, A1 |-i B1 : sSort z) /\
       (Σ ;;; Γ ,, A2 |-i B2 : sSort z) /\
-      (Σ ;;; Γ |-i u1 : sProd nx A1 B1) /\
-      (Σ ;;; Γ |-i u2 : sProd ny A2 B2) /\
+      (Σ ;;; Γ |-i u1 : sProd A1 B1) /\
+      (Σ ;;; Γ |-i u2 : sProd A2 B2) /\
       (Σ ;;; Γ |-i v1 : A1) /\
       (Σ ;;; Γ |-i v2 : A2) /\
-      (nl (sHeq (B1{0 := v1}) (sApp u1 A1 B1 v1)
-                (B2{0 := v2}) (sApp u2 A2 B2 v2))
-       = nl T).
+      (sHeq (B1{0 := v1}) (sApp u1 A1 B1 v1) (B2{0 := v2}) (sApp u2 A2 B2 v2) = T).
 Proof.
   invtac.
 Defined.
@@ -377,7 +364,7 @@ Defined.
 Lemma inversionCongSum :
   forall {Σ Γ B1 B2 pA pB T},
     Σ ;;; Γ |-i sCongSum B1 B2 pA pB : T ->
-    exists s z nx ny A1 A2,
+    exists s z A1 A2,
       (Σ ;;; Γ |-i pA : sHeq (sSort s) A1 (sSort s) A2) /\
       (Σ ;;; Γ ,, (sPack A1 A2)
        |-i pB : sHeq (sSort z) ((lift 1 1 B1){ 0 := sProjT1 (sRel 0) })
@@ -386,17 +373,15 @@ Lemma inversionCongSum :
       (Σ ;;; Γ |-i A2 : sSort s) /\
       (Σ ;;; Γ ,, A1 |-i B1 : sSort z) /\
       (Σ ;;; Γ ,, A2 |-i B2 : sSort z) /\
-      (nl (sHeq (sSort (Sorts.sum_sort s z)) (sSum nx A1 B1)
-                (sSort (Sorts.sum_sort s z)) (sSum ny A2 B2))
-       = nl T).
+      (sHeq (sSort (Sorts.sum_sort s z)) (sSum A1 B1) (sSort (Sorts.sum_sort s z)) (sSum A2 B2) = T).
 Proof.
-  invtac. Unshelve. all: constructor.
+  invtac.
 Defined.
 
 Lemma inversionCongPair :
   forall {Σ Γ B1 B2 pA pB pu pv T},
     Σ ;;; Γ |-i sCongPair B1 B2 pA pB pu pv : T ->
-    exists s z nx ny A1 A2 u1 u2 v1 v2,
+    exists s z A1 A2 u1 u2 v1 v2,
       (Σ ;;; Γ |-i pA : sHeq (sSort s) A1 (sSort s) A2) /\
       (Σ ;;; Γ ,, (sPack A1 A2)
        |-i pB : sHeq (sSort z) ((lift 1 1 B1){ 0 := sProjT1 (sRel 0) })
@@ -411,29 +396,27 @@ Lemma inversionCongPair :
       (Σ ;;; Γ |-i u2 : A2) /\
       (Σ ;;; Γ |-i v1 : B1{ 0 := u1 }) /\
       (Σ ;;; Γ |-i v2 : B2{ 0 := u2 }) /\
-      (nl (sHeq (sSum nx A1 B1) (sPair A1 B1 u1 v1)
-                (sSum ny A2 B2) (sPair A2 B2 u2 v2))
-       = nl T).
+      (sHeq (sSum A1 B1) (sPair A1 B1 u1 v1) (sSum A2 B2) (sPair A2 B2 u2 v2) = T).
 Proof.
-  invtac. Unshelve. all: constructor.
+  invtac.
 Defined.
 
 Lemma inversionCongPi1 :
   forall {Σ Γ B1 B2 pA pB pp T},
     Σ ;;; Γ |-i sCongPi1 B1 B2 pA pB pp : T ->
-    exists s z nx ny A1 A2 p1 p2,
+    exists s z A1 A2 p1 p2,
       (Σ ;;; Γ |-i pA : sHeq (sSort s) A1 (sSort s) A2) /\
       (Σ ;;; Γ ,, (sPack A1 A2)
        |-i pB : sHeq (sSort z) ((lift 1 1 B1){ 0 := sProjT1 (sRel 0) })
                     (sSort z) ((lift 1 1 B2){ 0 := sProjT2 (sRel 0) })) /\
-      (Σ ;;; Γ |-i pp : sHeq (sSum nx A1 B1) p1 (sSum ny A2 B2) p2) /\
+      (Σ ;;; Γ |-i pp : sHeq (sSum A1 B1) p1 (sSum A2 B2) p2) /\
       (Σ ;;; Γ |-i A1 : sSort s) /\
       (Σ ;;; Γ |-i A2 : sSort s) /\
       (Σ ;;; Γ ,, A1 |-i B1 : sSort z) /\
       (Σ ;;; Γ ,, A2 |-i B2 : sSort z) /\
-      (Σ ;;; Γ |-i p1 : sSum nx A1 B1) /\
-      (Σ ;;; Γ |-i p2 : sSum ny A2 B2) /\
-      (nl (sHeq A1 (sPi1 A1 B1 p1) A2 (sPi1 A2 B2 p2)) = nl T).
+      (Σ ;;; Γ |-i p1 : sSum A1 B1) /\
+      (Σ ;;; Γ |-i p2 : sSum A2 B2) /\
+      (sHeq A1 (sPi1 A1 B1 p1) A2 (sPi1 A2 B2 p2) = T).
 Proof.
   invtac.
 Defined.
@@ -441,21 +424,19 @@ Defined.
 Lemma inversionCongPi2 :
   forall {Σ Γ B1 B2 pA pB pp T},
     Σ ;;; Γ |-i sCongPi2 B1 B2 pA pB pp : T ->
-    exists s z nx ny A1 A2 p1 p2,
+    exists s z A1 A2 p1 p2,
       (Σ ;;; Γ |-i pA : sHeq (sSort s) A1 (sSort s) A2) /\
       (Σ ;;; Γ ,, (sPack A1 A2)
        |-i pB : sHeq (sSort z) ((lift 1 1 B1){ 0 := sProjT1 (sRel 0) })
                     (sSort z) ((lift 1 1 B2){ 0 := sProjT2 (sRel 0) })) /\
-      (Σ ;;; Γ |-i pp : sHeq (sSum nx A1 B1) p1 (sSum ny A2 B2) p2) /\
+      (Σ ;;; Γ |-i pp : sHeq (sSum A1 B1) p1 (sSum A2 B2) p2) /\
       (Σ ;;; Γ |-i A1 : sSort s) /\
       (Σ ;;; Γ |-i A2 : sSort s) /\
       (Σ ;;; Γ ,, A1 |-i B1 : sSort z) /\
       (Σ ;;; Γ ,, A2 |-i B2 : sSort z) /\
-      (Σ ;;; Γ |-i p1 : sSum nx A1 B1) /\
-      (Σ ;;; Γ |-i p2 : sSum ny A2 B2) /\
-      (nl (sHeq (B1{ 0 := sPi1 A1 B1 p1}) (sPi2 A1 B1 p1)
-                (B2{ 0 := sPi1 A2 B2 p2}) (sPi2 A2 B2 p2))
-       = nl T).
+      (Σ ;;; Γ |-i p1 : sSum A1 B1) /\
+      (Σ ;;; Γ |-i p2 : sSum A2 B2) /\
+      (sHeq (B1{ 0 := sPi1 A1 B1 p1}) (sPi2 A1 B1 p1) (B2{ 0 := sPi1 A2 B2 p2}) (sPi2 A2 B2 p2) = T).
 Proof.
   invtac.
 Defined.
@@ -473,9 +454,7 @@ Lemma inversionCongEq :
       (Σ ;;; Γ |-i u2 : A2) /\
       (Σ ;;; Γ |-i v1 : A1) /\
       (Σ ;;; Γ |-i v2 : A2) /\
-      (nl (sHeq (sSort (Sorts.eq_sort s)) (sEq A1 u1 v1)
-            (sSort (Sorts.eq_sort s)) (sEq A2 u2 v2))
-       = nl T).
+      (sHeq (sSort (Sorts.eq_sort s)) (sEq A1 u1 v1) (sSort (Sorts.eq_sort s)) (sEq A2 u2 v2) = T).
 Proof.
   invtac.
 Defined.
@@ -490,9 +469,7 @@ Lemma inversionCongRefl :
       (Σ ;;; Γ |-i A2 : sSort s) /\
       (Σ ;;; Γ |-i u1 : A1) /\
       (Σ ;;; Γ |-i u2 : A2) /\
-      (nl (sHeq (sEq A1 u1 u1) (sRefl A1 u1)
-                (sEq A2 u2 u2) (sRefl A2 u2))
-       = nl T).
+      (sHeq (sEq A1 u1 u1) (sRefl A1 u1) (sEq A2 u2 u2) (sRefl A2 u2) = T).
 Proof.
   invtac.
 Defined.
@@ -505,7 +482,7 @@ Lemma inversionEqToHeq :
       (Σ ;;; Γ |-i A : sSort s) /\
       (Σ ;;; Γ |-i u : A) /\
       (Σ ;;; Γ |-i v : A) /\
-      (nl (sHeq A u A v) = nl T).
+      (sHeq A u A v = T).
 Proof.
   invtac.
 Defined.
@@ -519,7 +496,7 @@ Lemma inversionHeqTypeEq :
       (Σ ;;; Γ |-i B : sSort s) /\
       (Σ ;;; Γ |-i u : A) /\
       (Σ ;;; Γ |-i v : B) /\
-      (nl (sEq (sSort s) A B) = nl T).
+      (sEq (sSort s) A B = T).
 Proof.
   invtac.
 Defined.
@@ -531,7 +508,7 @@ Lemma inversionProjT1 :
       (Σ ;;; Γ |-i p : sPack A1 A2) /\
       (Σ ;;; Γ |-i A1 : sSort s) /\
       (Σ ;;; Γ |-i A2 : sSort s) /\
-      (nl A1 = nl T).
+      (A1 = T).
 Proof.
   invtac.
 Defined.
@@ -543,7 +520,7 @@ Lemma inversionProjT2 :
       (Σ ;;; Γ |-i p : sPack A1 A2) /\
       (Σ ;;; Γ |-i A1 : sSort s) /\
       (Σ ;;; Γ |-i A2 : sSort s) /\
-      (nl A2 = nl T).
+      (A2 = T).
 Proof.
   invtac.
 Defined.
@@ -555,7 +532,7 @@ Lemma inversionProjTe :
       (Σ ;;; Γ |-i p : sPack A1 A2) /\
       (Σ ;;; Γ |-i A1 : sSort s) /\
       (Σ ;;; Γ |-i A2 : sSort s) /\
-      (nl (sHeq A1 (sProjT1 p) A2 (sProjT2 p)) = nl T).
+      (sHeq A1 (sProjT1 p) A2 (sProjT2 p) = T).
 Proof.
   invtac.
 Defined.
@@ -565,7 +542,7 @@ Lemma inversionAx :
     Σ ;;; Γ |-i sAx id : T ->
     exists ty,
       (lookup_glob Σ id = Some ty) /\
-      (nl ty = nl T).
+      (ty = T).
 Proof.
   invtac.
 Defined.
@@ -582,11 +559,6 @@ Ltac ttinv h :=
   let s2 := fresh "s2" in
   let z := fresh "z" in
   let his := fresh "is" in
-  let nx := fresh "nx" in
-  let ny := fresh "ny" in
-  let np := fresh "np" in
-  let ne := fresh "ne" in
-  let na := fresh "na" in
   let A := fresh "A" in
   let B := fresh "B" in
   let C := fresh "C" in
@@ -616,18 +588,16 @@ Ltac ttinv h :=
     lazymatch term with
     | sRel _ => destruct (inversionRel h) as [his [? ?]]
     | sSort _ => pose proof (inversionSort h) as hh
-    | sProd _ _ _ => destruct (inversionProd h) as (s1 & s2 & hh) ; splits_one hh
-    | sLambda _ _ _ _ => destruct (inversionLambda h) as (s1 & s2 & na & hh) ;
-                        splits_one hh
-    | sApp _ _ _ _ => destruct (inversionApp h) as (s1 & s2 & na & hh) ;
-                       splits_one hh
-    | sSum _ _ _ => destruct (inversionSum h) as (s1 & s2 & hh) ; splits_one hh
+    | sProd _ _ => destruct (inversionProd h) as (s1 & s2 & hh) ; splits_one hh
+    | sLambda _ _ _ => destruct (inversionLambda h) as (s1 & s2 & hh) ; splits_one hh
+    | sApp _ _ _ _ => destruct (inversionApp h) as (s1 & s2 & hh) ; splits_one hh
+    | sSum _ _ => destruct (inversionSum h) as (s1 & s2 & hh) ; splits_one hh
     | sPair _ _ _ _ =>
-      destruct (inversionPair h) as (nx & s1 & s2 & hh) ; splits_one hh
+      destruct (inversionPair h) as (s1 & s2 & hh) ; splits_one hh
     | sPi1 _ _ _ =>
-      destruct (inversionPi1 h) as (nx & s1 & s2 & hh) ; splits_one hh
+      destruct (inversionPi1 h) as (s1 & s2 & hh) ; splits_one hh
     | sPi2 _ _ _ =>
-      destruct (inversionPi2 h) as (nx & s1 & s2 & hh) ; splits_one hh
+      destruct (inversionPi2 h) as (s1 & s2 & hh) ; splits_one hh
     | sEq _ _ _ => destruct (inversionEq h) as (s & hh) ; splits_one hh
     | sRefl _ _ => destruct (inversionRefl h) as (s & hh) ; splits_one hh
     | sJ _ _ _ _ _ _ => destruct (inversionJ h) as (s1 & s2 & hh) ;
@@ -635,7 +605,7 @@ Ltac ttinv h :=
     | sTransport _ _ _ _ => destruct (inversionTransport h) as (s & hh) ;
                            splits_one hh
     | sBeta _ _ =>
-      destruct (inversionBeta h) as (s & nx & A & B & hh) ; splits_one hh
+      destruct (inversionBeta h) as (s & A & B & hh) ; splits_one hh
     | sHeq _ _ _ _ => destruct (inversionHeq h) as (s & hh) ; splits_one hh
     | sHeqToEq _ => destruct (inversionHeqToEq h) as (A & u & v & s & hh) ;
                    splits_one hh
@@ -649,30 +619,30 @@ Ltac ttinv h :=
       destruct (inversionHeqTransport h) as (A & B & s & hh) ;
       splits_one hh
     | sCongProd _ _ _ _ =>
-      destruct (inversionCongProd h) as (s & z & nx & ny & A1 & A2 & hh) ;
+      destruct (inversionCongProd h) as (s & z & A1 & A2 & hh) ;
       splits_one hh
     | sCongLambda _ _ _ _ _ _ _ =>
       destruct (inversionCongLambda h)
-        as (s & z & nx & ny & A1 & A2 & hh) ;
+        as (s & z & A1 & A2 & hh) ;
       splits_one hh
     | sCongApp _ _ _ _ _ _ =>
       destruct (inversionCongApp h)
-        as (s & z & nx & ny & A1 & A2 & u1 & u2 & v1 & v2 & hh) ;
+        as (s & z & A1 & A2 & u1 & u2 & v1 & v2 & hh) ;
       splits_one hh
     | sCongSum _ _ _ _ =>
-      destruct (inversionCongSum h) as (s & z & nx & ny & A1 & A2 & hh) ;
+      destruct (inversionCongSum h) as (s & z & A1 & A2 & hh) ;
       splits_one hh
     | sCongPair _ _ _ _ _ _ =>
       destruct (inversionCongPair h)
-        as (s & z & nx & ny & A1 & A2 & u1 & u2 & v1 & v2 & hh) ;
+        as (s & z & A1 & A2 & u1 & u2 & v1 & v2 & hh) ;
       splits_one hh
     | sCongPi1 _ _ _ _ _ =>
       destruct (inversionCongPi1 h)
-        as (s & z & nx & ny & A1 & A2 & p1 & p2 & hh) ;
+        as (s & z & A1 & A2 & p1 & p2 & hh) ;
       splits_one hh
     | sCongPi2 _ _ _ _ _ =>
       destruct (inversionCongPi2 h)
-        as (s & z & nx & ny & A1 & A2 & p1 & p2 & hh) ;
+        as (s & z & A1 & A2 & p1 & p2 & hh) ;
       splits_one hh
     | sCongEq _ _ _ =>
       destruct (inversionCongEq h) as (s & A1 & A2 & u1 & u2 & v1 & v2 & hh) ;
