theories/XTyping.v
@@ -7,11 +7,11 @@ Reserved Notation " Σ ;;; Γ '|-x' t ≡ u : T " (at level 50, Γ, t, u, T at n
 
 Open Scope s_scope.
 
+Declare Scope x_scope.
+
 Section XTyping.
 
 Context `{Sort_notion : Sorts.notion}.
-
-Declare Scope x_scope.
 
 Inductive typing (Σ : sglobal_context) (Γ : scontext) : sterm -> sterm -> Type :=
 | type_Rel n :
@@ -22,44 +22,44 @@ Inductive typing (Σ : sglobal_context) (Γ : scontext) : sterm -> sterm -> Type
 | type_Sort s :
     Σ ;;; Γ |-x (sSort s) : sSort (succ s)
 
-| type_Prod n t b s1 s2 :
+| type_Prod t b s1 s2 :
     Σ ;;; Γ |-x t : sSort s1 ->
     Σ ;;; Γ ,, t |-x b : sSort s2 ->
-    Σ ;;; Γ |-x (sProd n t b) : sSort (Sorts.prod_sort s1 s2)
+    Σ ;;; Γ |-x (sProd t b) : sSort (Sorts.prod_sort s1 s2)
 
-| type_Lambda n n' t b s1 s2 bty :
+| type_Lambda t b s1 s2 bty :
     Σ ;;; Γ |-x t : sSort s1 ->
     Σ ;;; Γ ,, t |-x bty : sSort s2 ->
     Σ ;;; Γ ,, t |-x b : bty ->
-    Σ ;;; Γ |-x (sLambda n t bty b) : sProd n' t bty
+    Σ ;;; Γ |-x (sLambda t bty b) : sProd t bty
 
-| type_App n s1 s2 t A B u :
+| type_App s1 s2 t A B u :
     Σ ;;; Γ |-x A : sSort s1 ->
     Σ ;;; Γ ,, A |-x B : sSort s2 ->
-    Σ ;;; Γ |-x t : sProd n A B ->
+    Σ ;;; Γ |-x t : sProd A B ->
     Σ ;;; Γ |-x u : A ->
     Σ ;;; Γ |-x (sApp t A B u) : B{ 0 := u }
 
-| type_Sum n t b s1 s2 :
+| type_Sum t b s1 s2 :
     Σ ;;; Γ |-x t : sSort s1 ->
     Σ ;;; Γ ,, t |-x b : sSort s2 ->
-    Σ ;;; Γ |-x (sSum n t b) : sSort (Sorts.sum_sort s1 s2)
+    Σ ;;; Γ |-x (sSum t b) : sSort (Sorts.sum_sort s1 s2)
 
-| type_Pair n A B u v s1 s2 :
+| type_Pair A B u v s1 s2 :
     Σ ;;; Γ |-x A : sSort s1 ->
     Σ ;;; Γ ,, A |-x B : sSort s2 ->
     Σ ;;; Γ |-x u : A ->
     Σ ;;; Γ |-x v : B{ 0 := u } ->
-    Σ ;;; Γ |-x sPair A B u v : sSum n A B
+    Σ ;;; Γ |-x sPair A B u v : sSum A B
 
-| type_Pi1 n A B s1 s2 p :
-    Σ ;;; Γ |-x p : sSum n A B ->
+| type_Pi1 A B s1 s2 p :
+    Σ ;;; Γ |-x p : sSum A B ->
     Σ ;;; Γ |-x A : sSort s1 ->
     Σ ;;; Γ ,, A |-x B : sSort s2 ->
     Σ ;;; Γ |-x sPi1 A B p : A
 
-| type_Pi2 n A B s1 s2 p :
-    Σ ;;; Γ |-x p : sSum n A B ->
+| type_Pi2 A B s1 s2 p :
+    Σ ;;; Γ |-x p : sSum A B ->
     Σ ;;; Γ |-x A : sSort s1 ->
     Σ ;;; Γ ,, A |-x B : sSort s2 ->
     Σ ;;; Γ |-x sPi2 A B p : B{ 0 := sPi1 A B p }
@@ -101,27 +101,27 @@ with eq_term (Σ : sglobal_context) (Γ : scontext) : sterm -> sterm -> sterm ->
     Σ ;;; Γ |-x v ≡ w : A ->
     Σ ;;; Γ |-x u ≡ w : A
 
-| eq_beta s1 s2 n A B t u :
+| eq_beta s1 s2 A B t u :
     Σ ;;; Γ |-x A : sSort s1 ->
     Σ ;;; Γ ,, A |-x B : sSort s2 ->
     Σ ;;; Γ ,, A |-x t : B ->
     Σ ;;; Γ |-x u : A ->
-    Σ ;;; Γ |-x sApp (sLambda n A B t) A B u ≡ t{ 0 := u } : B{ 0 := u }
+    Σ ;;; Γ |-x sApp (sLambda A B t) A B u ≡ t{ 0 := u } : B{ 0 := u }
 
 | eq_conv s T1 T2 t1 t2 :
     Σ ;;; Γ |-x t1 ≡ t2 : T1 ->
     Σ ;;; Γ |-x T1 ≡ T2 : sSort s ->
     Σ ;;; Γ |-x t1 ≡ t2 : T2
 
-| cong_Prod n1 n2 A1 A2 B1 B2 s1 s2 :
+| cong_Prod A1 A2 B1 B2 s1 s2 :
     Σ ;;; Γ |-x A1 ≡ A2 : sSort s1 ->
     Σ ;;; Γ ,, A1 |-x B1 ≡ B2 : sSort s2 ->
     Σ ;;; Γ ,, A1 |-x B1 : sSort s2 ->
     Σ ;;; Γ ,, A2 |-x B2 : sSort s2 ->
-    Σ ;;; Γ |-x (sProd n1 A1 B1) ≡ (sProd n2 A2 B2) :
+    Σ ;;; Γ |-x (sProd A1 B1) ≡ (sProd A2 B2) :
                sSort (Sorts.prod_sort s1 s2)
 
-| cong_Lambda n1 n2 n' A1 A2 B1 B2 t1 t2 s1 s2 :
+| cong_Lambda A1 A2 B1 B2 t1 t2 s1 s2 :
     Σ ;;; Γ |-x A1 ≡ A2 : sSort s1 ->
     Σ ;;; Γ ,, A1 |-x B1 ≡ B2 : sSort s2 ->
     Σ ;;; Γ ,, A1 |-x t1 ≡ t2 : B1 ->
@@ -129,29 +129,29 @@ with eq_term (Σ : sglobal_context) (Γ : scontext) : sterm -> sterm -> sterm ->
     Σ ;;; Γ ,, A2 |-x B2 : sSort s2 ->
     Σ ;;; Γ ,, A1 |-x t1 : B1 ->
     Σ ;;; Γ ,, A2 |-x t2 : B2 ->
-    Σ ;;; Γ |-x (sLambda n1 A1 B1 t1) ≡ (sLambda n2 A2 B2 t2) : sProd n' A1 B1
+    Σ ;;; Γ |-x (sLambda A1 B1 t1) ≡ (sLambda A2 B2 t2) : sProd A1 B1
 
-| cong_App n1 n2 s1 s2 t1 t2 A1 A2 B1 B2 u1 u2 :
+| cong_App s1 s2 t1 t2 A1 A2 B1 B2 u1 u2 :
     Σ ;;; Γ |-x A1 ≡ A2 : sSort s1 ->
     Σ ;;; Γ ,, A1 |-x B1 ≡ B2 : sSort s2 ->
-    Σ ;;; Γ |-x t1 ≡ t2 : sProd n1 A1 B1 ->
+    Σ ;;; Γ |-x t1 ≡ t2 : sProd A1 B1 ->
     Σ ;;; Γ |-x u1 ≡ u2 : A1 ->
     Σ ;;; Γ ,, A1 |-x B1 : sSort s2 ->
     Σ ;;; Γ ,, A2 |-x B2 : sSort s2 ->
-    Σ ;;; Γ |-x t1 : sProd n1 A1 B1 ->
-    Σ ;;; Γ |-x t2 : sProd n2 A2 B2 ->
+    Σ ;;; Γ |-x t1 : sProd A1 B1 ->
+    Σ ;;; Γ |-x t2 : sProd A2 B2 ->
     Σ ;;; Γ |-x u1 : A1 ->
     Σ ;;; Γ |-x u2 : A2 ->
     Σ ;;; Γ |-x (sApp t1 A1 B1 u1) ≡ (sApp t2 A2 B2 u2) : B1{ 0 := u1 }
 
-| cong_Sum n1 n2 A1 A2 B1 B2 s1 s2 :
+| cong_Sum A1 A2 B1 B2 s1 s2 :
     Σ ;;; Γ |-x A1 ≡ A2 : sSort s1 ->
     Σ ;;; Γ ,, A1 |-x B1 ≡ B2 : sSort s2 ->
     Σ ;;; Γ ,, A1 |-x B1 : sSort s2 ->
     Σ ;;; Γ ,, A2 |-x B2 : sSort s2 ->
-    Σ ;;; Γ |-x (sSum n1 A1 B1) ≡ (sSum n2 A2 B2) : sSort (Sorts.sum_sort s1 s2)
+    Σ ;;; Γ |-x (sSum A1 B1) ≡ (sSum A2 B2) : sSort (Sorts.sum_sort s1 s2)
 
-| cong_Pair n A1 A2 B1 B2 u1 u2 v1 v2 s1 s2 :
+| cong_Pair A1 A2 B1 B2 u1 u2 v1 v2 s1 s2 :
     Σ ;;; Γ |-x A1 ≡ A2 : sSort s1 ->
     Σ ;;; Γ ,, A1 |-x B1 ≡ B2 : sSort s2 ->
     Σ ;;; Γ |-x u1 ≡ u2 : A1 ->
@@ -162,26 +162,26 @@ with eq_term (Σ : sglobal_context) (Γ : scontext) : sterm -> sterm -> sterm ->
     Σ ;;; Γ |-x u2 : A2 ->
     Σ ;;; Γ |-x v1 : B1{ 0 := u1 } ->
     Σ ;;; Γ |-x v2 : B2{ 0 := u2 } ->
-    Σ ;;; Γ |-x sPair A1 B1 u1 v1 ≡ sPair A2 B2 u2 v2 : sSum n A1 B1
+    Σ ;;; Γ |-x sPair A1 B1 u1 v1 ≡ sPair A2 B2 u2 v2 : sSum A1 B1
 
-| cong_Pi1 nx ny A1 A2 B1 B2 s1 s2 p1 p2 :
-    Σ ;;; Γ |-x p1 ≡ p2 : sSum nx A1 B1 ->
+| cong_Pi1 A1 A2 B1 B2 s1 s2 p1 p2 :
+    Σ ;;; Γ |-x p1 ≡ p2 : sSum A1 B1 ->
     Σ ;;; Γ |-x A1 ≡ A2 : sSort s1 ->
     Σ ;;; Γ ,, A1 |-x B1 ≡ B2 : sSort s2 ->
     Σ ;;; Γ ,, A1 |-x B1 : sSort s2 ->
     Σ ;;; Γ ,, A2 |-x B2 : sSort s2 ->
-    Σ ;;; Γ |-x p1 : sSum nx A1 B1 ->
-    Σ ;;; Γ |-x p2 : sSum ny A2 B2 ->
+    Σ ;;; Γ |-x p1 : sSum A1 B1 ->
+    Σ ;;; Γ |-x p2 : sSum A2 B2 ->
     Σ ;;; Γ |-x sPi1 A1 B1 p1 ≡ sPi1 A2 B2 p2 : A1
 
-| cong_Pi2 nx ny A1 A2 B1 B2 s1 s2 p1 p2 :
-    Σ ;;; Γ |-x p1 ≡ p2 : sSum nx A1 B1 ->
+| cong_Pi2 A1 A2 B1 B2 s1 s2 p1 p2 :
+    Σ ;;; Γ |-x p1 ≡ p2 : sSum A1 B1 ->
     Σ ;;; Γ |-x A1 ≡ A2 : sSort s1 ->
     Σ ;;; Γ ,, A1 |-x B1 ≡ B2 : sSort s2 ->
     Σ ;;; Γ ,, A1 |-x B1 : sSort s2 ->
     Σ ;;; Γ ,, A2 |-x B2 : sSort s2 ->
-    Σ ;;; Γ |-x p1 : sSum nx A1 B1 ->
-    Σ ;;; Γ |-x p2 : sSum ny A2 B2 ->
+    Σ ;;; Γ |-x p1 : sSum A1 B1 ->
+    Σ ;;; Γ |-x p2 : sSum A2 B2 ->
     Σ ;;; Γ |-x sPi2 A1 B1 p1 ≡ sPi2 A2 B2 p2 : B1{ 0 := sPi1 A1 B1 p1 }
 
 | cong_Eq s A1 A2 u1 u2 v1 v2 :
@@ -197,11 +197,6 @@ with eq_term (Σ : sglobal_context) (Γ : scontext) : sterm -> sterm -> sterm ->
 
 | reflection A u v e :
     Σ ;;; Γ |-x e : sEq A u v ->
-    Σ ;;; Γ |-x u ≡ v : A
-
-| eq_alpha u v A :
-    nl u = nl v ->
-    Σ ;;; Γ |-x u : A ->
     Σ ;;; Γ |-x u ≡ v : A
 
 where " Σ ;;; Γ '|-x' t ≡ u : T " := (@eq_term Σ Γ t u T) : x_scope.
